\documentclass[11pt,a4paper]{article}
\usepackage{fullpage}
\usepackage{kpfonts,amsmath,booktabs}

\def\damped{_\text{d}}
\pagestyle{empty}

\begin{document}

\def\dampfactor{\phi_h}
\def\damped{$_{\text{d}}$}

\begin{small}\fontsize{7.9}{10}\rmfamily\tabcolsep=0.1cm
\begin{tabular}{clll}
\multicolumn{4}{l}{\it ADDITIVE ERROR MODELS}\\
\toprule
\bf Trend & \multicolumn{3}{c}{\bf Seasonal} \\
 & \multicolumn{1}{c}{\bf N}
 & \multicolumn{1}{c}{\bf A}
 & \multicolumn{1}{c}{\bf M} \\
\cmidrule{2-4}
{\bf N}
    & $y_{t} = \ell_{t-1}+\varepsilon_t$
    & $y_{t} = \ell_{t-1} + s_{t-m}+\varepsilon_t$
    & $y_{t} = \ell_{t-1} s_{t-m}+\varepsilon_t$ \\
    & $\ell_t = \ell_{t-1} + \alpha  \varepsilon_t$
    & $\ell_t = \ell_{t-1} + \alpha  \varepsilon_t$
    & $\ell_t = \ell_{t-1} + \alpha  \varepsilon_t/s_{t-m}$ \\
    &&$s_t = s_{t-m} + \gamma  \varepsilon_t$
    & $s_t = s_{t-m} + \gamma  \varepsilon_t/\ell_{t-1}$
\\
\midrule
    & $y_{t} = \ell_{t-1} + b_{t-1}+\varepsilon_t$
    & $y_{t} = \ell_{t-1} + b_{t-1} + s_{ t-m}+\varepsilon_t$
    & $y_{t} = (\ell_{t-1}+b_{t-1})s_{t-m}+\varepsilon_t$ \\
{\bf A}
    & $\ell_t = \ell_{t-1} + b_{t-1} + \alpha  \varepsilon_t$
    & $\ell_t = \ell_{t-1} + b_{t-1} + \alpha  \varepsilon_t$
    & $\ell_t = \ell_{t-1} + b_{t-1} + \alpha
    \varepsilon_t/s_{t-m}$ \\
    & $b_t = b_{t-1} + \beta  \varepsilon_t$
    & $b_t = b_{t-1} + \beta  \varepsilon_t$
    & $b_t = b_{t-1} + \beta  \varepsilon_t/s_{t-m}$ \\
    &
    & $s_t =  s_{t-m} + \gamma  \varepsilon_t$
    & $s_t =  s_{t-m} + \gamma  \varepsilon_t/(\ell_{t-1}+b_{t-1})$
\\
\midrule
    & $y_{t} =  \ell_{t-1} + \phi b_{t-1}+\varepsilon_t$
    & $y_{t} =  \ell_{t-1} + \phi b_{t-1} + s_{t-m}+\varepsilon_t$
    & $y_{t} = (\ell_{t-1} + \phi b_{t-1})s_{t-m}+\varepsilon_t$ \\
{\bf A\damped }
    & $\ell_t = \ell_{t-1} + \phi b_{t-1} + \alpha  \varepsilon_t$
    & $\ell_t = \ell_{t-1} + \phi b_{t-1} + \alpha  \varepsilon_t$
    & $\ell_t = \ell_{t-1} + \phi b_{t-1} + \alpha
    \varepsilon_t/s_{t-m}$ \\
    & $b_t = \phi b_{t-1} + \beta  \varepsilon_t$
    & $b_t = \phi b_{t-1} + \beta  \varepsilon_t$
    & $b_t = \phi b_{t-1} + \beta  \varepsilon_t/s_{t-m}$ \\
    &
    & $s_t =  s_{t-m} + \gamma  \varepsilon_t$
    & $s_t =  s_{t-m} + \gamma  \varepsilon_t/(\ell_{t-1}+\phi
    b_{t-1})$
\\
\bottomrule\\
\multicolumn{4}{l}{\it MULTIPLICATIVE ERROR MODELS}\\
\toprule
\bf Trend & \multicolumn{3}{c}{\bf Seasonal} \\
 & \multicolumn{1}{c}{\bf N}
 & \multicolumn{1}{c}{\bf A}
 & \multicolumn{1}{c}{\bf M} \\
\cmidrule{2-4}
{\bf N}
    & $y_{t} = \ell_{t-1}(1 + \varepsilon_t)$
    & $y_{t} = (\ell_{t-1} + s_{t-m})(1 + \varepsilon_t)$
    & $y_{t} = \ell_{t-1} s_{t-m}(1 + \varepsilon_t)$ \\
    & $\ell_t = \ell_{t-1}(1 + \alpha \varepsilon_t)$
    & $\ell_t = \ell_{t-1} + \alpha(\ell_{t-1} + s_{t-m})
    \varepsilon_t$
    & $\ell_t = \ell_{t-1}(1 + \alpha \varepsilon_t)$ \\
    &&$s_t = s_{t-m} + \gamma  (\ell_{t-1} + s_{t-m})\varepsilon_t$
    & $s_t = s_{t-m}(1 + \gamma  \varepsilon_t)$
\\
\midrule
    & $y_{t} = (\ell_{t-1} + b_{t-1})(1 + \varepsilon_t)$
    & $y_{t} = (\ell_{t-1} + b_{t-1} + s_{ t-m})(1 + \varepsilon_t)$
    & $y_{t} = (\ell_{t-1}+b_{t-1})s_{t-m}(1 + \varepsilon_t)$ \\
{\bf A}
    & $\ell_t = (\ell_{t-1} + b_{t-1})(1 + \alpha  \varepsilon_t)$
    & $\ell_t = \ell_{t-1} + b_{t-1} + \alpha (\ell_{t-1} + b_{t-1}+ s_{ t-m}) \varepsilon_t$
    & $\ell_t = (\ell_{t-1} + b_{t-1})(1 + \alpha\varepsilon_t)$ \\
    & $b_t = b_{t-1} + \beta (\ell_{t-1} + b_{t-1}) \varepsilon_t$
    & $b_t = b_{t-1} + \beta (\ell_{t-1} + b_{t-1} + s_{ t-m})\varepsilon_t$
    & $b_t = b_{t-1} + \beta (\ell_{t-1}+b_{t-1})\varepsilon_t$ \\
    &
    & $s_t =  s_{t-m} + \gamma (\ell_{t-1} + b_{t-1} + s_{ t-m})\varepsilon_t$
    & $s_t =  s_{t-m}(1 + \gamma \varepsilon_t)$
\\
\midrule
    & $y_{t} =  (\ell_{t-1} + \phi b_{t-1})(1 + \varepsilon_t)$
    & $y_{t} =  (\ell_{t-1} + \phi b_{t-1} + s_{t-m})(1 + \varepsilon_t)$
    & $y_{t} = (\ell_{t-1} + \phi b_{t-1})s_{t-m}(1 + \varepsilon_t)$ \\
{\bf A\damped }
    & $\ell_t = (\ell_{t-1} + \phi b_{t-1})(1 + \alpha \varepsilon_t)$
    & $\ell_t = \ell_{t-1} + \phi b_{t-1} + \alpha (\ell_{t-1}+ \phi b_{t-1} + s_{t-m}) \varepsilon_t$
    & $\ell_t = (\ell_{t-1} + \phi b_{t-1})(1 + \alpha \varepsilon_t)$ \\
    & $b_t = \phi b_{t-1} + \beta(\ell_{t-1} + \phi b_{t-1})\varepsilon_t$
    & $b_t = \phi b_{t-1} + \beta  (\ell_{t-1} + \phi b_{t-1} +s_{t-m})\varepsilon_t$
    & $b_t = \phi b_{t-1} + \beta (\ell_{t-1} + \phi b_{t-1})\varepsilon_t$ \\
    &
    & $s_t =  s_{t-m} + \gamma (\ell_{t-1} + \phi b_{t-1} + s_{t-m})\varepsilon_t$
    & $s_t =  s_{t-m}(1+ \gamma \varepsilon_t)$
\\
\bottomrule
\end{tabular}\vspace{0.5cm}
\end{small}


\end{document}
